more proof rules

program_proof_rules.thy
@@ -49,6 +49,7 @@ definition execution_s_check where
        \<longrightarrow> currentProc S1 i \<triangleq> toImpl
        \<longrightarrow> visibleCalls S1 i \<triangleq>  vis
        \<longrightarrow> currentTransaction S1 i = tx
+       \<longrightarrow> (\<forall>tx'. tx \<noteq> Some tx' \<longrightarrow> transactionStatus S1 tx' \<noteq> Some Uncommitted)
        \<longrightarrow> traceCorrect_s  trace)"
 
 lemma beforeInvoc_execution_s_check: 
@@ -77,11 +78,11 @@ text "It is sufficient to check with @{term execution_s_check} to ensure that th
 lemma execution_s_check_sound:
   assumes  "localState S i \<triangleq> ls"
     and "visibleCalls S i \<triangleq> vis"
-    and "localState S i \<triangleq> ls"
     and "prog S = progr"
     and "currentProc S i \<triangleq> toImpl"
     and "generatedLocal = {x. generatedIds S x \<triangleq> i}"
     and "state_wellFormed S"
+    and no_uncommitted: "\<And>tx'. currentTransaction S i \<noteq> Some tx' \<longrightarrow> transactionStatus S tx' \<noteq> Some Uncommitted"
     and c: "execution_s_check 
   progr 
   i
@@ -108,28 +109,88 @@ proof (auto simp add:  execution_s_correct_def)
   show "traceCorrect_s  trace"
   proof (rule c[simplified execution_s_check_def, rule_format]; force?)
     show "state_wellFormed S"
-      by (simp add: assms(7))
+      by (simp add: assms)
 
     show "\<And>p t. (AInvoc p, t) \<notin> set trace"
-      using a0 assms(1) assms(7) no_more_invoc by blast
+      using a0 assms no_more_invoc by blast
 
 
     show "prog S = progr"
-      by (simp add: assms(4))
+      by (simp add: assms)
 
     show " generatedLocal = {x. generatedIds S x \<triangleq> i}"
-      by (auto simp add: assms(6))
+      by (auto simp add: assms)
 
     show "localState S i \<triangleq> ls"
       by (simp add: assms(1))
 
     show "currentProc S i \<triangleq> toImpl"
-      by (simp add: assms(5))
+      by (simp add: assms)
 
     show "visibleCalls S i \<triangleq> vis"
-      by (simp add: assms(2))
+      by (simp add: assms)
+
+
+    show "currentTransaction S i \<noteq> Some tx' \<Longrightarrow> transactionStatus S tx' \<noteq> Some Uncommitted" for tx'
+      by (simp add: assms)
+
   qed
 qed
+
+
+lemma execution_s_check_sound2:
+  assumes a1: "localState S i \<triangleq> ls"
+    and a2: "S \<in> initialStates progr i"
+    and a3: "currentProc S i \<triangleq> toImpl"
+    and c: "\<And>s_calls s_happensBefore s_callOrigin s_transactionOrigin s_knownIds s_invocationOp s_invocationRes.
+  execution_s_check 
+  progr 
+  i
+  s_calls
+  s_happensBefore
+  s_callOrigin
+  s_transactionOrigin
+  s_knownIds
+  s_invocationOp
+  s_invocationRes
+  {}
+  {}
+  None
+  ls"
+  shows "execution_s_correct progr S i"
+  using a1
+proof (rule execution_s_check_sound)
+
+
+  show "visibleCalls S i \<triangleq> {}"
+    using a2 by (auto simp add: initialStates_def)
+
+  show "prog S = progr"
+    using a2 by (auto simp add: initialStates_def)
+
+  show "currentProc S i \<triangleq> toImpl"
+    using a3 by simp
+
+  show wf: "state_wellFormed S"
+    using a2 initialStates_wellFormed by blast
+
+  show "{} = {x. generatedIds S x \<triangleq> i}"
+    using a2 wf_generated_ids_invocation_exists by (auto simp add: initialStates_def, blast)
+
+  have currentTx: "currentTransaction S i = None"
+    using a2 initialState_noTxns2 by blast
+
+
+  show "execution_s_check progr i (calls S) (happensBefore S) (callOrigin S) (transactionOrigin S) (knownIds S) (invocationOp S)
+     (invocationRes S) {} {} (currentTransaction S i) ls "
+    unfolding currentTx
+    by (rule c)
+
+  show "\<And>tx'. currentTransaction S i \<noteq> Some tx' \<longrightarrow> transactionStatus S tx' \<noteq> Some Uncommitted"
+    using a2 initialState_noTxns1 by blast
+
+qed
+
 
 lemma traceCorrect_s_empty: "traceCorrect_s  [] "
   by (simp add: traceCorrect_s_def) 
@@ -186,7 +247,8 @@ lemma execution_s_check_single_step:
   currentProc S1 i \<triangleq> toImpl;
   visibleCalls S1 i \<triangleq>  vis;
   currentTransaction S1 i = tx;
-  state_wellFormed S1
+  state_wellFormed S1;
+  \<And>tx'. tx \<noteq> Some tx' \<Longrightarrow>  transactionStatus S1 tx' \<noteq> Some Uncommitted
 \<rbrakk> \<Longrightarrow> 
   Inv
 \<and> (case localState S' i of
@@ -230,8 +292,9 @@ next
   case (Some action)
 
   show ?thesis
-  proof (auto simp add: execution_s_check_def)
-    fix trace S1 S'
+  proof (auto simp add: execution_s_check_def, goal_cases "A")
+    case (A trace S1 S')
+    (*fix trace S1 S'
     assume a0: "S1 ~~ (i, trace) \<leadsto>\<^sub>S* S'"
       and a1: "\<forall>p t. (AInvoc p, t) \<notin> set trace"
       and a2: "state_wellFormed S1"
@@ -247,7 +310,8 @@ next
       and a12: "localState S1 i \<triangleq> ls"
       and a13: "currentProc S1 i \<triangleq> toImpl"
       and a14: "visibleCalls S1 i \<triangleq> vis"
-      and a15: "tx = currentTransaction S1 i"
+      and a15: "tx = currentTransaction S1 i"*)
+
 
     show "traceCorrect_s  trace"
     proof (cases trace)
@@ -268,13 +332,13 @@ next
 
 
       have gI: "\<forall>x\<in>generatedLocal. generatedIds S1 x \<triangleq> i"
-        using a11 by blast
+        using A by blast
 
       have hasInvoc: "invocationOp S1 i \<noteq> None"
-        using Some a8 by auto
+        using Some A by auto
 
       have wf: "state_wellFormed S1"
-        using a2 by auto
+        using A by auto
 
 
       from step
@@ -283,7 +347,7 @@ next
      | Some LS' \<Rightarrow>
          execution_s_check progr i (calls S1') (happensBefore S1') (callOrigin S1') (transactionOrigin S1') (knownIds S1') (invocationOp S1')
           (invocationRes S1') {x. generatedIds S1' x \<triangleq> i} (visibleCalls S1' i orElse {}) (currentTransaction S1' i) LS')"
-        by (rule H; (simp add: a3 a4 a5 a6 a7 a8 a9 a10 a11 a12 a13 a14 a15 hasInvoc wf )?)
+        by (rule H; (simp add: A hasInvoc wf )?)
 
 
 
@@ -303,7 +367,7 @@ next
 
           with steps have "trace' = []"
             using local_state_None_no_more_steps
-            by (metis a0 a12 a2 insert_iff list.simps(15) local.Cons no_more_invoc option.simps(3)) 
+            by (metis A insert_iff list.simps(15) local.Cons no_more_invoc option.simps(3)) 
 
 
           then show ?thesis
@@ -322,21 +386,26 @@ next
           proof (rule execution_s_check_def[THEN meta_eq_to_obj_eq, THEN iffD1, rule_format])
             show "S1' ~~ (i, trace') \<leadsto>\<^sub>S* S'" using steps .
             show "\<And>p t. (AInvoc p, t) \<notin> set trace'"
-              using Some a2 local.step no_more_invoc state_wellFormed_combine_s1 steps by fastforce
+              using Some local.step local.wf no_more_invoc state_wellFormed_combine_s1 steps by fastforce
             show "state_wellFormed S1'"
-              using a2 local.step state_wellFormed_combine_s1 by blast
+              using A local.step state_wellFormed_combine_s1 by blast
             show "prog S1' = progr"
-              by (metis a0 a10 steps unchangedProg)
+              by (metis A steps unchangedProg)
             show "localState S1' i \<triangleq> LS'"
               by (simp add: Some)
 
 
 
             show "currentProc S1' i \<triangleq> toImpl"
-              using step Some a13 by (auto simp add: step_s.simps a12 a2 wf_localState_to_invocationOp)
+              using step Some by (auto simp add: step_s.simps A wf_localState_to_invocationOp)
 
             show "visibleCalls S1' i \<triangleq> visibleCalls S1' i orElse {}"
-              using step a14 Some  by (auto simp add: step_s.simps a12 a2 wf_localState_to_invocationOp split: option.splits)
+              using step  Some  by (auto simp add: step_s.simps A wf_localState_to_invocationOp split: option.splits)
+
+            show "\<And>tx'. currentTransaction S1' i \<noteq> Some tx' \<Longrightarrow> transactionStatus S1' tx' \<noteq> Some Uncommitted"
+              using step Some  by (auto simp add: step_s.simps A wf_localState_to_invocationOp split: option.splits if_splits)
+
+
 
           qed auto
         qed
@@ -399,22 +468,21 @@ definition
   "new_unique_not_in_calls_result iop uidv \<equiv>
 \<forall>i op r. iop i \<triangleq> Call op r \<longrightarrow> to_nat uidv \<notin> uniqueIds r "
 
+definition
+"new_unique_not_in_invocationRes ires uidv \<equiv> 
+\<forall>i r. ires i \<triangleq> r \<longrightarrow> to_nat uidv \<notin> uniqueIds r "
+
+
 lemma execution_s_check_newId:
   assumes "infinite (Collect P)"
     and "program_wellFormed progr"
-    (* TODO add properties about uniqueness of v:
-  - not in calls
-  - not in ops/results
-  - not known
-  - not generated in current 
-*)
     and cont: "\<And>v. \<lbrakk>P v; 
  new_unique_not_in_calls s_calls v;
 new_unique_not_in_calls_result s_calls v;
 new_unique_not_in_invocationOp s_invocationOp v;
 new_unique_not_in_invocationRes s_invocationRes v;
-new_unique_not_in_knownIds s_knownIds v;
-new_unique_not_generated_in_current localGenerated v;
+to_nat v \<notin> s_knownIds;
+to_nat v \<notin> localGenerated;
 uniqueIds v = {to_nat v}
 \<rbrakk> \<Longrightarrow> execution_s_check
   progr 
@@ -454,15 +522,9 @@ proof (rule  execution_s_check_single_step, auto simp add: step_s.simps split: i
       using `localGenerated = {x. generatedIds S1 x \<triangleq> i}` by auto
 
     show "new_unique_not_in_invocationOp s_invocationOp uidv"
-      apply (auto simp add: new_unique_not_in_invocationOp_def)
-      
-      sorry
+      using assms(2) goal(12) goal(14) goal(18) goal(5) new_unique_not_in_invocationOp_def wf_onlyGeneratedIdsInInvocationOps by blast
     show "new_unique_not_in_invocationRes s_invocationRes uidv"
-      sorry
-    show "new_unique_not_in_knownIds s_knownIds uidv"
-      sorry
-    show "new_unique_not_generated_in_current localGenerated uidv"
-      sorry
+      using assms(2) goal(13) goal(14) goal(18) goal(5) new_unique_not_in_invocationRes_def wf_onlyGeneratedIdsInInvocationRes by blast
     have "to_nat uidv \<notin> uniqueIds opr" if "calls S1 c \<triangleq> Call opr r" for c opr r
     proof (rule wf_onlyGeneratedIdsInCalls)
       show "calls S1 c \<triangleq> Call opr r" using that .
@@ -470,24 +532,223 @@ proof (rule  execution_s_check_single_step, auto simp add: step_s.simps split: i
         by (simp add: goal(5)) 
 
       show "program_wellFormed (prog S1)"
-        using assms(2) goal(13) by blast
+        using assms(2) goal(14) by blast
 
       show "generatedIds S1 (to_nat uidv) = None"
-        by (simp add: goal(17))
+        by (simp add: goal(18))
     qed
 
     from this
     show " new_unique_not_in_calls s_calls uidv"
-      by (simp add: goal(6) new_unique_not_in_calls_def)
+      by (simp add: goal(7) new_unique_not_in_calls_def)
 
     show " new_unique_not_in_calls_result s_calls uidv"
-      sorry
+      using assms(2) goal(14) goal(18) goal(5) goal(7) new_unique_not_in_calls_result_def wf_onlyGeneratedIdsInCallResults by blast
+
+    show "to_nat uidv \<notin> s_knownIds"
+      using assms(2) goal(11) goal(14) goal(18) goal(5) wf_onlyGeneratedIdsInKnownIds by blast
+
   qed
 qed
 
 
+lemma restrict_map_noop: "dom m \<subseteq> S \<Longrightarrow> m |` S = m"
+   using domIff by (auto simp add: restrict_map_def intro!: ext, force)
 
 
+lemma restrict_map_noop2[simp]: "m |` dom m = m"
+  by (simp add: restrict_map_noop)
+
+lemma restrict_relation_noop: "Field r \<subseteq> S \<Longrightarrow> r |r S = r"
+  by (auto simp add: restrict_relation_def FieldI1 FieldI2 subset_h1)
+
+
+lemma execution_s_check_beginAtomic:
+  assumes "tx = None"
+    and "program_wellFormed progr"
+    and cont: "\<And>tx s_calls' s_happensBefore' s_callOrigin' s_transactionOrigin' s_knownIds' vis'
+ s_invocationOp' s_invocationRes'.
+\<lbrakk>invariant progr
+     \<lparr>calls = s_calls', 
+      happensBefore = s_happensBefore',
+      callOrigin = s_callOrigin',
+      transactionOrigin = s_transactionOrigin', 
+      knownIds = s_knownIds',
+      invocationOp = s_invocationOp', 
+      invocationRes = s_invocationRes'\<rparr>
+\<comment> \<open>
+TODO: 
+- no calls in new transaction
+- state-growing predicates
+- vis growing
+- valid snapshot (causally + transactionally)
+- nothing happens on invocation i
+\<close>
+
+\<rbrakk> \<Longrightarrow> execution_s_check
+  progr 
+  i
+  s_calls' 
+  s_happensBefore' 
+  s_callOrigin' 
+  (s_transactionOrigin'(tx \<mapsto> i))
+  s_knownIds' 
+  s_invocationOp'
+  s_invocationRes'
+  localGenerated
+  vis'
+  (Some tx)
+  (cont ())"
+
+
+shows"execution_s_check
+  progr 
+  i
+  s_calls
+  s_happensBefore 
+  s_callOrigin
+  s_transactionOrigin 
+  s_knownIds
+  s_invocationOp
+  s_invocationRes
+  localGenerated
+  vis
+  tx
+  (beginAtomic \<bind> cont)
+"
+proof (rule  execution_s_check_single_step, auto simp add: step_s.simps split: if_splits, goal_cases "goal")
+  case (goal S1 Inv y t S'a vis')
+  show ?case 
+  proof (rule back_subst13[where P=execution_s_check], rule cont; (rule refl)?)
+    show "localGenerated = {x. generatedIds S'a x \<triangleq> i}"
+      apply (auto simp add: goal)
+      using `state_monotonicGrowth i S1 S'a` state_monotonicGrowth_generatedIds apply blast
+      using goal(21) state_monotonicGrowth_generatedIds_same1 by blast
+
+    have [simp]: "(prog S1) = progr"
+      by (simp add: goal(14))
+
+    show "progr = prog S1" by simp
+
+    have [simp]: "committedCalls S'a = dom(calls S'a)"
+      using committedCallsH_def committedCalls_allCommitted
+        `\<forall>x. transactionStatus S'a x \<noteq> Some Uncommitted`
+        `state_wellFormed S'a`
+      by (fastforce)
+
+    show "invariant progr
+     \<lparr>calls = calls S'a, happensBefore = happensBefore S'a, callOrigin = callOrigin S'a,
+        transactionOrigin = transactionOrigin S'a, knownIds = knownIds S'a, invocationOp = invocationOp S'a,
+        invocationRes = invocationRes S'a\<rparr>"
+      using `invariant (prog S1) (invContext S'a)`
+    proof (auto simp add: invContextH_def elim!: back_subst[where P="invariant progr"])
+      
+      show "\<And>a b. (a, b) \<in> happensBefore S'a |r dom (calls S'a) \<Longrightarrow> (a, b) \<in> happensBefore S'a"
+        by (simp add: restrict_relation_def)
+      show "\<And>a b. (a, b) \<in> happensBefore S'a \<Longrightarrow> (a, b) \<in> happensBefore S'a |r dom (calls S'a)"
+        by (simp add: goal(25) happensBefore_in_calls_left happensBefore_in_calls_right restrict_relation_def)
+      show "callOrigin S'a |` dom (calls S'a) = callOrigin S'a"
+        by (simp add: goal(25) restrict_map_noop wellFormed_callOrigin_dom)
+
+      show "transactionOrigin S'a |` committedTransactions S'a = transactionOrigin S'a"
+      proof (rule restrict_map_noop)
+        show "dom (transactionOrigin S'a) \<subseteq> committedTransactions S'a"
+          apply auto
+          by (metis (no_types, lifting) goal(25) goal(24) option.exhaust option.simps(3) transactionStatus.exhaust wf_transactionOrigin_and_status)
+      qed
+    qed
+  qed
+qed
+
+
+lemma execution_s_check_endAtomic:
+  assumes "tx \<noteq> None"
+    and "program_wellFormed progr"
+and assert_inv: "invariant progr 
+     \<lparr>calls = s_calls, 
+      happensBefore = s_happensBefore,
+      callOrigin = s_callOrigin,
+      transactionOrigin = s_transactionOrigin, 
+      knownIds = s_knownIds,
+      invocationOp = s_invocationOp, 
+      invocationRes = s_invocationRes\<rparr>"
+    and cont: "
+\<comment> \<open>
+
+\<close>
+\<lbrakk>True
+\<rbrakk> \<Longrightarrow> execution_s_check
+  progr 
+  i
+  s_calls 
+  s_happensBefore 
+  s_callOrigin 
+  s_transactionOrigin
+  s_knownIds 
+  s_invocationOp
+  s_invocationRes
+  localGenerated
+  vis
+  None
+  (cont ())"
+
+
+shows"execution_s_check
+  progr 
+  i
+  s_calls
+  s_happensBefore 
+  s_callOrigin
+  s_transactionOrigin 
+  s_knownIds
+  s_invocationOp
+  s_invocationRes
+  localGenerated
+  vis
+  tx
+  (endAtomic \<bind> cont)
+"
+proof (rule  execution_s_check_single_step, auto simp add: step_s.simps split: if_splits, goal_cases "inv" "goal")
+  case (inv S1 y t)
+
+  have [simp]: "prog S1 = progr" using inv by simp
+
+  have all_committed: "transactionStatus S1 tx \<triangleq> Committed"
+    if "tx \<noteq> t" 
+      and "callOrigin S1 x \<triangleq> tx"
+    for tx x
+    apply (case_tac "transactionStatus S1 tx")
+     apply auto
+    using inv(5) that(2) wf_no_transactionStatus_origin_for_nothing apply blast
+    using inv(6) that(1) transactionStatus.exhaust by force
+
+  have committedCalls_simp: "committedCallsH (callOrigin S1) (transactionStatus S1(t \<mapsto> Committed)) = dom s_calls"
+    apply (auto simp add: committedCallsH_def isCommittedH_def all_committed)
+    using inv(5) inv(7) wellFormed_callOrigin_dom apply fastforce
+      apply (simp add: inv(5) inv(7) wellFormed_callOrigin_dom2)
+    using inv(17) inv(5) not_uncommitted_cases wellFormed_currentTransaction_unique_h(2) apply blast
+    by (metis all_committed inv(5) inv(7) option.exhaust option.simps(3) wf_callOrigin_and_calls)
+
+  show ?case
+  proof (simp add: invContextH_def, rule back_subst[where P="invariant progr", OF assert_inv], auto simp add: inv committedCalls_simp)
+    show "\<And>a b. (a, b) \<in> happensBefore S1 \<Longrightarrow> (a, b) \<in> happensBefore S1 |r dom (calls S1)"
+      by (simp add: happensBefore_in_calls_left happensBefore_in_calls_right inv(5) restrict_relation_def)
+    show "\<And>a b. (a, b) \<in> happensBefore S1 |r dom (calls S1) \<Longrightarrow> (a, b) \<in> happensBefore S1"
+      by (simp add: happensBefore_in_calls_left happensBefore_in_calls_right inv(5) restrict_relation_def)
+
+    show "callOrigin S1 = callOrigin S1 |` dom (calls S1)"
+      by (metis inv(5) restrict_map_noop2 wellFormed_callOrigin_dom)
+
+    show "transactionOrigin S1 = transactionOrigin S1 |` {ta. ta \<noteq> t \<longrightarrow> transactionStatus S1 ta \<triangleq> Committed}"
+      apply (subst restrict_map_noop, auto)
+      by (metis  inv(5) inv(6) not_uncommitted_cases option.exhaust option.simps(3) wf_transactionOrigin_and_status)
+  qed
+next
+  case (goal S1 y t)
+  show ?case 
+  proof (rule back_subst13[where P=execution_s_check], rule cont; (simp add: goal)?)
+  qed
+qed
 
 
 
