execution_invariants2.thy
@@ -8,6 +8,20 @@ lemma wf_transaction_status_iff_origin_dom:
   shows "dom (transactionOrigin S) = dom (transactionStatus S)"
   by (smt Collect_cong dom_def local.wf wf_transaction_status_iff_origin)
 
+lemma wf_generated_ids_invocation_exists:
+  assumes wf: "state_wellFormed S"
+and "invocationOp S i = None"
+shows "generatedIds S uid \<noteq> Some i"
+  find_theorems name: induct state_wellFormed
+  using assms proof (induct rule: wellFormed_induct)
+  case initial
+  then show ?case by (simp add: initialState_def)
+next
+  case (step t a s)
+  then show ?case by (auto simp add: initialState_def step.simps wf_localState_to_invocationOp split: if_splits)
+qed
+
+
 
 
 end
