unique_ids.thy
@@ -3,7 +3,7 @@ theory unique_ids
 begin
 
 inductive procedure_cannot_guess_ids :: "uniqueId set \<Rightarrow> 'ls \<Rightarrow> ('ls, 'operation::valueType, 'any::valueType) procedureImpl \<Rightarrow> bool"  where
-pcgi_local:  "\<lbrakk>impl ls = LocalStep ls'; procedure_cannot_guess_ids uids ls' impl\<rbrakk> \<Longrightarrow>  procedure_cannot_guess_ids uids ls impl"
+  pcgi_local:  "\<lbrakk>impl ls = LocalStep ls'; procedure_cannot_guess_ids uids ls' impl\<rbrakk> \<Longrightarrow>  procedure_cannot_guess_ids uids ls impl"
 | pcgi_beginAtomic: "\<lbrakk>impl ls = BeginAtomic ls'; procedure_cannot_guess_ids uids ls' impl\<rbrakk> \<Longrightarrow>  procedure_cannot_guess_ids uids ls impl"
 | pcgi_endAtomic:"\<lbrakk>impl ls = EndAtomic ls'; procedure_cannot_guess_ids uids ls' impl\<rbrakk> \<Longrightarrow>  procedure_cannot_guess_ids uids ls impl"
 | pcgi_newId:"\<lbrakk>impl ls = NewId f; \<And>uid ls'. f uid \<triangleq> ls' \<Longrightarrow> procedure_cannot_guess_ids (uids \<union> uniqueIds uid) ls' impl
@@ -32,8 +32,8 @@ lemma pcgi_return_case:"\<lbrakk>procedure_cannot_guess_ids uids ls impl; impl l
 
 lemma procedure_cannot_guess_ids_mono:
   assumes "procedure_cannot_guess_ids uids ls impl"
-and "uids \<subseteq> uids'"
-shows "procedure_cannot_guess_ids uids' ls impl"
+    and "uids \<subseteq> uids'"
+  shows "procedure_cannot_guess_ids uids' ls impl"
   using assms apply (induct  arbitrary: uids uids' rule: procedure_cannot_guess_ids.induct)
        apply (auto simp add: procedure_cannot_guess_ids.intros)
     apply (meson procedure_cannot_guess_ids.intros(4) sup.cobounded1)
@@ -48,18 +48,18 @@ shows "procedure_cannot_guess_ids uids' ls impl"
 
 
 definition procedures_cannot_guess_ids :: "('proc::valueType \<Rightarrow> ('ls \<times> ('ls, 'operation::valueType, 'any::valueType) procedureImpl)) \<Rightarrow> bool" where
-"procedures_cannot_guess_ids proc = 
+  "procedures_cannot_guess_ids proc = 
 (\<forall>p ls impl uids. proc p = (ls, impl) \<longrightarrow>  procedure_cannot_guess_ids (uids\<union>uniqueIds p) ls impl)"
 
 lemmas show_procedures_cannot_guess_ids = procedures_cannot_guess_ids_def[THEN iffD1, rule_format]
 
 definition query_cannot_guess_ids :: "uniqueId set \<Rightarrow> (('operation::valueType, 'any::valueType) operationContext \<Rightarrow> 'any \<Rightarrow> bool) \<Rightarrow> bool"  where
-"query_cannot_guess_ids oprUids spec \<equiv> 
+  "query_cannot_guess_ids oprUids spec \<equiv> 
   \<forall>ctxt res. 
    spec ctxt res \<longrightarrow> uniqueIds res \<subseteq> oprUids \<union> \<Union>{uniqueIds (call_operation c) | cId c. calls ctxt cId \<triangleq> c}"
 
 lemma query_cannot_guess_ids_def2:
-"query_cannot_guess_ids oprUids spec =
+  "query_cannot_guess_ids oprUids spec =
   (\<forall>ctxt res x. 
    spec ctxt res 
  \<longrightarrow> x \<in> uniqueIds res 
@@ -73,12 +73,12 @@ lemma query_cannot_guess_ids_def2:
   by (metis call.sel(1))
 
 definition queries_cannot_guess_ids :: "('operation \<Rightarrow> ('operation::valueType, 'any::valueType) operationContext \<Rightarrow> 'any \<Rightarrow> bool) \<Rightarrow> bool"  where
-"queries_cannot_guess_ids spec \<equiv> 
+  "queries_cannot_guess_ids spec \<equiv> 
   \<forall>opr. query_cannot_guess_ids (uniqueIds opr) (spec opr)"
 
 
 lemma queries_cannot_guess_ids_def2:
-"queries_cannot_guess_ids qry =
+  "queries_cannot_guess_ids qry =
   (\<forall>opr ctxt res x. 
    qry opr ctxt res 
  \<longrightarrow> x \<in> uniqueIds res 
@@ -88,13 +88,13 @@ lemma queries_cannot_guess_ids_def2:
 
 
 definition program_wellFormed :: " ('proc::valueType, 'ls, 'operation::valueType, 'any::valueType) prog \<Rightarrow> bool" where
-"program_wellFormed progr \<equiv> 
+  "program_wellFormed progr \<equiv> 
    procedures_cannot_guess_ids (procedure progr)
  \<and> queries_cannot_guess_ids (querySpec progr)
 "
 
 lemma exists_elim_h: "\<lbrakk>P x; Q x\<rbrakk> \<Longrightarrow> \<exists>x. P x \<and> Q x" for P Q x
-    by auto
+  by auto
 
 
 
@@ -105,6 +105,7 @@ lemma wf_knownIds_subset_generatedIds_h:
   shows "\<And>i ls impl. localState S i \<triangleq> ls \<Longrightarrow> currentProc S i \<triangleq> impl \<Longrightarrow> \<exists>uids\<subseteq>dom (generatedIds S). procedure_cannot_guess_ids uids ls impl"
     and "knownIds S \<subseteq> dom (generatedIds S)"
     and "\<And>c opr r. calls S c \<triangleq> Call opr r \<Longrightarrow> uniqueIds opr \<subseteq> dom (generatedIds S)"
+    and "\<And>c opr r. calls S c \<triangleq> Call opr r \<Longrightarrow> uniqueIds r \<subseteq> dom (generatedIds S)"
 
   using wf prog_wf
 proof -
@@ -114,7 +115,7 @@ proof -
   have H: "(\<forall>i ls impl. localState S i \<triangleq> ls \<and> currentProc S i \<triangleq> impl
       \<longrightarrow> (\<exists>uids. uids \<subseteq> dom (generatedIds S) \<and> procedure_cannot_guess_ids uids ls impl))
        \<and> (knownIds S \<subseteq> dom (generatedIds S))
-       \<and> (\<forall>c opr r. calls S c \<triangleq> Call opr r \<longrightarrow> uniqueIds opr \<subseteq> dom (generatedIds S))"
+       \<and> (\<forall>c opr r. calls S c \<triangleq> Call opr r \<longrightarrow> uniqueIds opr \<subseteq> dom (generatedIds S) \<and> uniqueIds r \<subseteq> dom (generatedIds S))"
   proof (induct rule: wellFormed_induct)
     case initial
     then show ?case by (simp add: initialState_def)
@@ -300,6 +301,86 @@ proof -
         by (auto simp add: step.simps split: if_splits;
             meson domD in_mono inv1 pcgi_dbop_case1 | blast
             )
+      hence call_ops_unique: "x\<in>dom(generatedIds S2)"
+        if "x\<in>uniqueIds opr" and "calls S2 c \<triangleq> Call opr r"
+        for  c opr r x
+        using that by blast
+
+      have query_no_guess: " query_cannot_guess_ids (uniqueIds opr) (querySpec progr opr)" for opr
+        using \<open>queries_cannot_guess_ids (querySpec progr)\<close>
+        by (auto simp add:  queries_cannot_guess_ids_def)
+
+      have query_no_guess2: "\<exists>cId opr r. x \<in> uniqueIds opr \<and> calls ctxt cId \<triangleq> Call opr r"
+        if "x\<in>uniqueIds res" 
+          and " querySpec progr opr ctxt res "
+          and "x\<notin> uniqueIds opr"
+        for x res opr ctxt
+        using that 
+        by (metis (no_types, lifting) \<open>queries_cannot_guess_ids (querySpec progr)\<close> queries_cannot_guess_ids_def2) 
+
+      have "x \<in> dom (generatedIds S2)"
+        if c0: "calls S2 c \<triangleq> Call opr r"
+          and c1: "x\<in>uniqueIds r"
+        for  c opr r x
+
+        using `S1 ~~ a \<leadsto> S2` that
+      proof (cases rule: step.cases)
+        case (dbop i ls f Op ls' t c' res vis)
+
+        have "generatedIds S1 = generatedIds S2"
+          using dbop by auto
+
+        have "calls S2 c' \<triangleq> Call Op res"
+          using dbop by auto
+
+        from dbop show ?thesis
+          using c0 c1 proof (auto split: if_splits, goal_cases "A" "B")
+          case A
+          have "calls S2 c \<triangleq> Call opr r"
+            using A by auto
+
+
+          have "x \<in> dom (generatedIds S2)" if "x \<in> uniqueIds opr"
+            using call_ops_unique[OF `x \<in> uniqueIds opr` `calls S2 c \<triangleq> Call opr r`] by simp
+          hence "x \<in> dom (generatedIds S1)" if "x \<in> uniqueIds opr"
+            using \<open>generatedIds S1 = generatedIds S2\<close> that by auto
+
+
+
+          show ?case
+          proof (rule ccontr, auto)
+            assume "generatedIds S1 x = None"
+            hence "x \<notin> uniqueIds opr"
+              using \<open>generatedIds S1 = generatedIds S2\<close> \<open>x \<in> uniqueIds opr \<Longrightarrow> x \<in> dom (generatedIds S2)\<close> by auto
+
+            from query_no_guess2[OF `x \<in> uniqueIds r` `querySpec progr opr (getContextH (calls S1) (happensBefore S1) (Some vis)) r` `x \<notin> uniqueIds opr`]
+            obtain cId opr' r'
+              where "x \<in> uniqueIds opr'"
+                and c: "calls S1 cId \<triangleq> Call opr' r'"
+              by (auto simp add: getContextH_def restrict_map_def split: if_splits)
+
+
+
+
+            from inv3[OF c]
+            have "uniqueIds opr' \<subseteq> dom (generatedIds S1)"
+              by blast
+
+
+            show False
+              using \<open>generatedIds S1 x = None\<close> \<open>uniqueIds opr' \<subseteq> dom (generatedIds S1)\<close> \<open>x \<in> uniqueIds opr'\<close> by blast
+          qed
+        next
+          case B
+          show ?case
+            using B(12) \<open>prog S1 = progr\<close> c1 prog_wf step.hyps(2) by blast
+        qed
+      qed (insert c0 c1  \<open>prog S1 = progr\<close> prog_wf step.hyps(2), auto simp add: step.simps split: if_splits; blast)+
+
+      thus "uniqueIds r \<subseteq> dom (generatedIds S2)"
+        if c0: "calls S2 c \<triangleq> Call opr r"
+        for  c opr r
+        using that by blast
     qed
   qed
 
@@ -310,6 +391,9 @@ proof -
        \<lbrakk>localState S i \<triangleq> ls; currentProc S i \<triangleq> impl; state_wellFormed S; program_wellFormed (prog S)\<rbrakk>
        \<Longrightarrow> \<exists>uids\<subseteq>dom (generatedIds S). procedure_cannot_guess_ids uids ls impl"
     "\<And>c opr r. \<lbrakk>calls S c \<triangleq> Call opr r; state_wellFormed S; program_wellFormed (prog S)\<rbrakk> \<Longrightarrow> uniqueIds opr \<subseteq> dom (generatedIds S)"
+    "\<And>c opr r.
+       \<lbrakk>calls S c \<triangleq> Call opr r; state_wellFormed S; program_wellFormed (prog S)\<rbrakk>
+       \<Longrightarrow> uniqueIds r \<subseteq> dom (generatedIds S)"
     by blast+
 
 qed
@@ -347,6 +431,51 @@ lemma wf_onlyGeneratedIdsInCalls:
   shows "calls S c \<triangleq> Call opr r \<Longrightarrow> uid \<notin> uniqueIds opr"
   by (meson domIff in_mono local.wf not_generated prog_wf wf_knownIds_subset_generatedIds_h(3))
 
+
+lemma wf_onlyGeneratedIdsInCallResults:
+  fixes S :: "('proc::valueType, 'ls, 'operation::valueType, 'any::valueType) state"
+  assumes wf: "state_wellFormed S"
+    and prog_wf: "program_wellFormed (prog S)"
+    and not_generated: "generatedIds S uid = None"
+  shows "calls S c \<triangleq> Call opr r \<Longrightarrow> uid \<notin> uniqueIds r"
+  by (meson domIff in_mono local.wf not_generated prog_wf wf_knownIds_subset_generatedIds_h(4))
+
+lemma wf_onlyGeneratedIdsInInvocationOps:
+  fixes S :: "('proc::valueType, 'ls, 'operation::valueType, 'any::valueType) state"
+  assumes wf: "state_wellFormed S"
+    and prog_wf: "program_wellFormed (prog S)"
+    and not_generated: "generatedIds S uid = None"
+  shows "invocationOp S c \<triangleq> opr \<Longrightarrow> uid \<notin> uniqueIds opr"
+  using wf prog_wf not_generated proof (induct rule: wellFormed_induct)
+  case initial
+  then show ?case 
+    by (auto simp add: initialState_def)
+
+next
+  case (step t a s)
+  then show ?case 
+    apply (auto simp add: step.simps split: if_splits, goal_cases "new_invoc")
+    using wf_onlyGeneratedIdsInKnownIds by blast
+qed
+
+lemma wf_onlyGeneratedIdsInInvocationRes:
+  fixes S :: "('proc::valueType, 'ls, 'operation::valueType, 'any::valueType) state"
+  assumes wf: "state_wellFormed S"
+    and prog_wf: "program_wellFormed (prog S)"
+    and not_generated: "generatedIds S uid = None"
+  shows "invocationRes S c \<triangleq> res \<Longrightarrow> uid \<notin> uniqueIds res"
+  using wf prog_wf not_generated proof (induct rule: wellFormed_induct)
+  case initial
+  then show ?case 
+    by (auto simp add: initialState_def)
+
+next
+  case (step t a s)
+  then show ?case 
+    apply (auto simp add: step.simps split: if_splits, goal_cases "new_invoc")
+    by (smt domIff pcgi_return_case subset_iff wf_knownIds_subset_generatedIds_h(1))
+
+qed
 
 
 
